lakefile.lean
@@ -4,6 +4,9 @@ open Lake DSL
 package «fp-course» where
   name := "fp-course"
 
+require mathlib from git
+  "https://github.com/leanprover-community/mathlib4.git" @ "v4.28.0"
+
 @[default_target]
 lean_lib «FPCourse» where
   globs := #[.andSubmodules `FPCourse]
